\documentclass{article}
\usepackage[utf8]{inputenc}
\usepackage{amssymb}
\usepackage{amsmath}
\usepackage{mathrsfs}
%espacement de ligne
\usepackage{setspace}
\renewcommand{\baselinestretch}{1.5} 
% Graphiques et figures
\usepackage{float}
\usepackage{graphicx}
%avoir des subfigures 
\usepackage{caption}
\usepackage{subcaption}
%entourer une figure
\usepackage{wrapfig}
\begin{document}

\section*{Résumé}

\begin{align*}
S=\int{d^2x[\frac{1}{2} (\frac{\partial \psi}{\partial x})^2 + \frac{1}{2} (\frac{\partial \phi}{\partial x})^2 -V(\phi,\psi)]}
\end{align*}

\begin{align*}
\text{Solution statique:}& (\psi_o, \phi_o) \\
\text{Solution déformée:}& (\psi_o, \xi(t)(\phi_o(x)+1)-1) \\
\end{align*}

\begin{align*}
S=&\int{d^2x[\frac{1}{2}\dot{\xi}^2(\phi_o(x)+1)^2 - \left(\frac{1}{2}\xi^2\phi_o'^2 + \frac{1}{2}\psi_o'^2 +V(\phi_o,\psi_o,\xi(t))\right)]} \\
=&\int{dt\left[\frac{1}{2}\dot{\xi}^2\underbrace{\int{dx  (\phi_o(x)+1)^2}}_M -\underbrace{\left( \xi^2\int{dx\phi_o'^2}+\int{dx\psi_o'^2}+\int{dxV(\phi_o,\psi_o,\xi(t))}\right)}_{U(\xi)}\right]} \\
S=&\int{dt [\frac{1}{2}M \dot{\xi}^2 - U(\xi)]}
\end{align*}
par Euler-Lagrange:

\begin{align*}
\frac{1}{2}M \dot{\xi}^2 = U \\
F(\xi) \equiv \dot{\xi} = \sqrt{2 U(\xi)/M}\\
S_E =& \int{dt[M\dot{\xi}^2]}\\
=& \int{dt[M F(\xi) \dot{\xi}]} \\
=& \int_{1}^{\xi o} \mathrm{d}\xi [\sqrt{2M} \hat{F}(\xi)]\\
\hat{F}=\sqrt{\xi^2\int{dx\phi_o'^2}+\int{dx\psi_o'^2}+\int{dxV(\phi_o,\psi_o,\xi(t))}}
\end{align*}


\begin{align*}
V(\phi,\psi)=(\psi^2-\delta_1)(\psi^2-1)^2 + \frac{\alpha}{\psi^2+\gamma}\left[(\phi^2-1)^2 - \frac{\delta_2}{4}(\phi-2)(\phi+1)^2 \right] \\
f \equiv \xi(\phi_o +1)\\
V(f,\psi_o) = (\psi^2-\delta_1)(\psi^2-1)^2+\frac{\alpha}{\psi^2+\gamma}\left[(f^2-2f)^2 -\frac{\delta_2}{4}(f-3)f^2 \right]\\
\int{dxV(\phi_o,\psi_o,\xi(t))} = \int{dx[\psi^2-\delta_1)(\psi^2-1)^2]} \
+\alpha\xi^2\left[& \xi^2\int{dx[\frac{(\phi_o+1)^4}{\psi_o^2+\gamma}]} \
-\xi(4+\frac{\delta_2}{4})\int{dx[\frac{(\phi_o+1)^3}{\psi_o^2+\gamma}]} \\
& +(4+\frac{3\delta_2}{4})\int{dx[\frac{(\phi_o+1)^2}{\psi_o^2+\gamma}]} \
\right] \\
\end{align*}

\end{document}
